example_Patterns.thy
@@ -1,19 +1,52 @@
 theory example_Patterns imports Patterns
  begin
-definition P1_inv where "P1_inv t t1_0 A1 A2' A3' s \<equiv> (always_inv (\<lambda> r2 r1 . ((\<not> (A1 r1)) \<or> (constrained_until_inv t t1_0 A2' A3' r2 r1))) s)"
+definition P1 where "P1 t A1 A2 A3 s \<equiv> (always (\<lambda> r2 r1 . ((\<not> (A1 r1)) \<or> (constrained_until t A2 A3 r2 r1))) s)"
+
+definition example_part where "example_part t A1 A2 A3 s \<equiv> (P1 t A1 (\<lambda> s s1 . (A2 s1)) (\<lambda> s s1 . (A3 s1)) s)"
+
+definition P1_inv where "P1_inv t t1_0 A1 A2_1 A3_1 s \<equiv> (always_inv (\<lambda> r2 r1 . ((\<not> (A1 r1)) \<or> (constrained_until_inv t t1_0 A2_1 A3_1 r2 r1))) s)"
+
+definition P1_inv_part_inv where "P1_inv_part_inv t t1_0 A1 A2 A3 s \<equiv> (P1_inv t t1_0 A1 (\<lambda> s s1 . (A2 s1)) (\<lambda> s s1 . (A3 s1)) s)"
 
 
-lemma P1_inv_saving : "
-P1_inv t t1_0 A1 A2' A3' s0 \<Longrightarrow>
-consecutive s0 s
-((True \<or> ((A2' s0) \<and> ((A3' s0) \<and> ((t1_0 s0) \<or> (((A3' s s) \<and> ((t1_0 s0) <= t)) \<or> ((A2' s s) \<and> ((t1_0 s0) < (t1_0 s)))))))) \<and> ((\<not> (A1 s)) \<or> (constrained_until_inv t t1_0 A2' A3' s s)))
-P1_inv t t1_0 A1 A2' A3' s"
 
-lemma P1_inv_saving : "
-P1_inv t t1_0 A1 A2' A3' s0 \<Longrightarrow>
-toEnvP s0
-(True \<or> ((A2' s) \<and> ((A3' s) \<and> ((t1_0 s) <= t))))
+lemma P1_inv_saving_gen: "
+P1_inv t t1_0 A1 A2_1 A3_1 s0 \<Longrightarrow>
+consecutive s0 s \<Longrightarrow>
+((True \<and> ((always_imp s0 (A2_1 s0) (A2_1 s)) \<and> ((always_imp s0 (A3_1 s0) (A3_1 s)) \<and> (((t1_0 s0) = 0) \<or> (((A3_1 s s) \<and> ((t1_0 s0) <= t)) \<or> ((A2_1 s s) \<and> ((t1_0 s0) < (t1_0 s)))))))) \<and> ((\<not> (A1 s)) \<or> ((A3_1 s s) \<or> ((A2_1 s s) \<and> ((t1_0 s) > 0))))) \<Longrightarrow>
+P1_inv t t1_0 A1 A2_1 A3_1 s"
+  unfolding P1_inv_def
+  apply proveOuter
+  done
+
+lemma P1einv_imp_req_gen: "
+P1_inv t t1_0 A1 A2_1 A3_1 s0 \<Longrightarrow>
+toEnvP s0 \<Longrightarrow>
+(True \<and> ((always_imp s0 (A2_1 s0) (A2 s0)) \<and> ((always_imp s0 (A3_1 s0) (A3 s0)) \<and> ((t1_0 s0) <= t)))) \<Longrightarrow>
 P1 t A1 A2 A3 s0"
+  unfolding P1_inv_def P1_def
+  apply proveOuter
+  done
+
+lemma P1_inv_saving: "
+P1_inv_part_inv t t1_0 A1 A2 A3 s0 \<Longrightarrow>
+consecutive s0 s \<Longrightarrow>
+((((t1_0 s0) = 0) \<or> (((A3 s) \<and> ((t1_0 s0) <= t)) \<or> ((A2 s) \<and> ((t1_0 s0) < (t1_0 s))))) \<and> ((\<not> (A1 s)) \<or> ((A3 s) \<or> ((A2 s) \<and> ((t1_0 s) > 0))))) \<Longrightarrow>
+P1_inv_part_inv t t1_0 A1 A2 A3 s"
+  unfolding P1_inv_part_inv_def
+  apply(auto intro: P1_inv_saving_gen  always_imp_refl)
+  done
+
+lemma P1einv_imp_req: "
+P1_inv_part_inv t t1_0 A1 A2 A3 s0 \<Longrightarrow>
+toEnvP s0 \<Longrightarrow>
+((t1_0 s) <= t) \<Longrightarrow>
+example_part t A1 A2 A3 s0"
+  unfolding P1_inv_part_inv_def example_part_def
+  apply(erule P1einv_imp_req_gen)
+   apply(auto simp add: always_imp_refl)
+
+lemmas P1_used_patterns = always constrained_until 
 
 lemmas P1_inv_used_patterns = always_inv constrained_until_inv 
 
