Weak_Until.thy
@@ -12,7 +12,7 @@ definition weak_until_inv where "weak_until_inv w A1 A2 s s1 \<equiv>
 (\<forall> s2. toEnvP s2 \<and> s1 \<le> s2 \<and> s2 < s3 \<longrightarrow> A1 s s2)) \<or>
 w s \<and> (\<forall> s2. toEnvP s2 \<and> s1 \<le> s2 \<and> s2 \<le> s \<longrightarrow> A1 s s2)"
 
-lemma weak_until_rule: "consecutive s0 s \<Longrightarrow>
+lemma weak_until_rule[patternintro]: "consecutive s0 s \<Longrightarrow>
 always_imp s0 (A1' s0) (A1' s) \<and>
 always_imp s0 (A2' s0) (A2' s) \<and>
 (\<not> w s0 \<or>  A2' s s \<or> w s \<and> A1' s s) \<Longrightarrow>
@@ -20,12 +20,12 @@ always_imp s0 (weak_until_inv w A1' A2' s0) (weak_until_inv w A1' A2' s)"
   unfolding weak_until_inv_def  less_eq_state.simps less_state.simps always_imp_def
   by (smt (verit, best) consecutive.elims(2) substate_noteq_imp_substate_of_pred substate_refl substate_trans)
 
-lemma weak_until_one_point: "toEnvP s \<Longrightarrow> A2 s s \<or> w s \<and> A1 s s \<Longrightarrow> weak_until_inv w A1 A2  s s"
+lemma weak_until_one_point[patternintro]: "toEnvP s \<Longrightarrow> A2 s s \<or> w s \<and> A1 s s \<Longrightarrow> weak_until_inv w A1 A2  s s"
   apply(unfold weak_until_inv_def)
   unfolding weak_until_inv_def  less_eq_state.simps less_state.simps
   using substate_antisym substate_refl by blast
 
-lemma weak_until_einv2req: "
+lemma weak_until_einv2req[patternintro]: "
 always_imp s (A1' s) (A1 s) \<and>
 always_imp s (A2' s) (A2 s) \<Longrightarrow>
 always_imp s (weak_until_inv w A1' A2' s) (weak_until A1 A2 s)"
