Always.thy~
@@ -2,19 +2,19 @@ theory Always
   imports RequirementLemmas
 begin
 
-definition always where "always (s::state) s1 A \<equiv>
+definition always where "always A (s::state) s1 \<equiv>
 \<forall> r1. r1 \<le> s1 \<and> toEnvP r1 \<longrightarrow> A s r1"
 
-definition always_inv where "always_inv s A' \<equiv>
+definition always_inv where "always_inv A' s \<equiv>
 \<forall> r1. r1 \<le> s \<and> toEnvP r1 \<longrightarrow> A' s r1"
 
-lemma always_rule[elims]: "always_inv s A' \<Longrightarrow> consecutive s s' \<Longrightarrow>  always_imp s (A' s) (A' s') \<and> A' s' s' \<Longrightarrow>
- always_inv s' A'"
+lemma always_rule[elims]: "always_inv A' s \<Longrightarrow> consecutive s s' \<Longrightarrow>  always_imp s (A' s) (A' s') \<and> A' s' s' \<Longrightarrow>
+ always_inv A' s'"
   apply(unfold always_inv_def always_imp_def)
   apply simp
   by (metis One_nat_def substate_noteq_imp_substate_of_pred)
 
-lemma always_einv2req[elims]: "always_inv s A'  \<Longrightarrow> toEnvP s \<Longrightarrow> always_imp s (A' s) (A s) \<Longrightarrow> always s s A"
+lemma always_einv2req[elims]: "always_inv A' s  \<Longrightarrow> toEnvP s \<Longrightarrow> always_imp s (A' s) (A s) \<Longrightarrow> always A s s"
   apply(unfold always_def always_inv_def always_imp_def)
   by simp
 
